theories/TM/LM/JumpTargetTM.v
@@ -16,25 +16,25 @@ Definition retr_nat_prog : Retract sigNat sigPro := Retract_sigList_X _.
 
 
 (** append a token to the token list *)
-Definition App_Tokens : pTM sigPro^+ (FinType(EqType unit)) 2 :=
+Definition App_Comens : pTM sigPro^+ (FinType(EqType unit)) 2 :=
   App' _ @ [|Fin0; Fin1|];;
   MoveValue _ @ [|Fin1; Fin0|].
 
-Definition App_Tokens_Rel : pRel sigPro^+ (FinType(EqType unit)) 2 :=
+Definition App_Comens_Rel : pRel sigPro^+ (FinType(EqType unit)) 2 :=
   ignoreParam (
       fun tin tout =>
-        forall (Q Q' : list Tok),
+        forall (Q Q' : list Com),
           tin[@Fin0] ≃ Q ->
           tin[@Fin1] ≃ Q' ->
           tout[@Fin0] ≃ Q ++ Q' /\
           isRight tout[@Fin1]
     ).
 
-Lemma App_Tokens_Realise : App_Tokens ⊨ App_Tokens_Rel.
+Lemma App_Comens_Realise : App_Comens ⊨ App_Comens_Rel.
 Proof.
   eapply Realise_monotone.
-  { unfold App_Tokens. TM_Correct.
-    - apply App'_Realise with (X := Tok).
+  { unfold App_Comens. TM_Correct.
+    - apply App'_Realise with (X := Com).
     - apply MoveValue_Realise with (X := Pro).
   }
   {
@@ -44,17 +44,17 @@ Proof.
 Qed.
 
 
-Definition App_Tokens_steps (Q Q': Pro) := 1 + App'_steps _ Q + MoveValue_steps _ _ (Q ++ Q') Q.
+Definition App_Comens_steps (Q Q': Pro) := 1 + App'_steps _ Q + MoveValue_steps _ _ (Q ++ Q') Q.
 
-Definition App_Tokens_T : tRel sigPro^+ 2 :=
-  fun tin k => exists (Q Q' : list Tok), tin[@Fin0] ≃ Q /\ tin[@Fin1] ≃ Q' /\ App_Tokens_steps Q Q' <= k.
+Definition App_Comens_T : tRel sigPro^+ 2 :=
+  fun tin k => exists (Q Q' : list Com), tin[@Fin0] ≃ Q /\ tin[@Fin1] ≃ Q' /\ App_Comens_steps Q Q' <= k.
 
-Lemma App_Tokens_Terminates : projT1 App_Tokens ↓ App_Tokens_T.
+Lemma App_Comens_Terminates : projT1 App_Comens ↓ App_Comens_T.
 Proof.
   eapply TerminatesIn_monotone.
-  { unfold App_Tokens. TM_Correct.
-    - apply App'_Realise with (X := Tok).
-    - apply App'_Terminates with (X := Tok).
+  { unfold App_Comens. TM_Correct.
+    - apply App'_Realise with (X := Com).
+    - apply App'_Terminates with (X := Com).
     - apply MoveValue_Terminates with (X := Pro) (Y := Pro).
   }
   {
@@ -68,64 +68,64 @@ Qed.
 
 
 (** append a token to the token list *)
-Definition App_ATok (t : ATok) : pTM sigPro^+ unit 2 :=
-  WriteValue (encode [ATok2Tok t]) @ [|Fin1|];;
-  App_Tokens.
+Definition App_ACom (t : ACom) : pTM sigPro^+ unit 2 :=
+  WriteValue (encode [ACom2Com t]) @ [|Fin1|];;
+  App_Comens.
 
-Definition App_ATok_Rel (t : ATok) : pRel sigPro^+ unit 2 :=
+Definition App_ACom_Rel (t : ACom) : pRel sigPro^+ unit 2 :=
   ignoreParam (
       fun tin tout =>
-        forall (Q : list Tok),
+        forall (Q : list Com),
           tin[@Fin0] ≃ Q ->
           isRight tin[@Fin1] ->
-          tout[@Fin0] ≃ Q ++ [ATok2Tok t] /\
+          tout[@Fin0] ≃ Q ++ [ACom2Com t] /\
           isRight tout[@Fin1]
     ).
 
-Lemma App_ATok_Realise t : App_ATok t ⊨ App_ATok_Rel t.
+Lemma App_ACom_Realise t : App_ACom t ⊨ App_ACom_Rel t.
 Proof.
   eapply Realise_monotone.
-  { unfold App_ATok. TM_Correct.
-    - apply App_Tokens_Realise.
+  { unfold App_ACom. TM_Correct.
+    - apply App_Comens_Realise.
   }
   {
     intros tin ((), tout) H. intros Q HENcQ HRight1.
-    TMSimp. specialize (H [ATok2Tok t] eq_refl). modpon H. modpon H0. auto.
+    TMSimp. specialize (H [ACom2Com t] eq_refl). modpon H. modpon H0. auto.
   }
 Qed.
 
-Definition App_ATok_steps (Q: Pro) (t: ATok) := 1 + WriteValue_steps (size _ [ATok2Tok t]) + App_Tokens_steps Q [ATok2Tok t].
+Definition App_ACom_steps (Q: Pro) (t: ACom) := 1 + WriteValue_steps (size _ [ACom2Com t]) + App_Comens_steps Q [ACom2Com t].
 
-Definition App_ATok_T (t: ATok) : tRel sigPro^+ 2 :=
-  fun tin k => exists (Q: list Tok), tin[@Fin0] ≃ Q /\ isRight tin[@Fin1] /\ App_ATok_steps Q t <= k.
+Definition App_ACom_T (t: ACom) : tRel sigPro^+ 2 :=
+  fun tin k => exists (Q: list Com), tin[@Fin0] ≃ Q /\ isRight tin[@Fin1] /\ App_ACom_steps Q t <= k.
 
-Lemma App_ATok_Terminates (t: ATok) : projT1 (App_ATok t) ↓ App_ATok_T t.
+Lemma App_ACom_Terminates (t: ACom) : projT1 (App_ACom t) ↓ App_ACom_T t.
 Proof.
   eapply TerminatesIn_monotone.
-  { unfold App_ATok. TM_Correct.
-    - apply App_Tokens_Terminates.
+  { unfold App_ACom. TM_Correct.
+    - apply App_Comens_Terminates.
   }
   {
     intros tin k. intros (Q&HEncQ&HRight&Hk).
-    exists (WriteValue_steps (size _ [ATok2Tok t])), (App_Tokens_steps Q [ATok2Tok t]). cbn; repeat split; try omega.
+    exists (WriteValue_steps (size _ [ACom2Com t])), (App_Comens_steps Q [ACom2Com t]). cbn; repeat split; try omega.
     now rewrite Hk.
-    intros tmid () (HWrite&HInjWrite); hnf; cbn; TMSimp. specialize (HWrite [ATok2Tok t] eq_refl). modpon HWrite. eauto.
+    intros tmid () (HWrite&HInjWrite); hnf; cbn; TMSimp. specialize (HWrite [ACom2Com t] eq_refl). modpon HWrite. eauto.
   }
 Qed.
 
 
 
 (** Add a singleton list of tokes to [Q] *)
-Definition App_Tok : pTM sigPro^+ (FinType(EqType unit)) 3 :=
+Definition App_Com : pTM sigPro^+ (FinType(EqType unit)) 3 :=
   Constr_nil _ @ [|Fin2|];;
   Constr_cons _@ [|Fin2; Fin1|];;
-  App_Tokens @ [|Fin0; Fin2|];;
+  App_Comens @ [|Fin0; Fin2|];;
   Reset _ @ [|Fin1|].
 
-Definition App_Tok_Rel : pRel sigPro^+ (FinType(EqType unit)) 3 :=
+Definition App_Com_Rel : pRel sigPro^+ (FinType(EqType unit)) 3 :=
   ignoreParam (
       fun tin tout =>
-        forall (Q : list Tok) (t : Tok),
+        forall (Q : list Com) (t : Com),
           tin[@Fin0] ≃ Q ->
           tin[@Fin1] ≃ t ->
           isRight tin[@Fin2] ->
@@ -135,42 +135,42 @@ Definition App_Tok_Rel : pRel sigPro^+ (FinType(EqType unit)) 3 :=
     ).
 
 
-Lemma App_Tok_Realise : App_Tok ⊨ App_Tok_Rel.
+Lemma App_Com_Realise : App_Com ⊨ App_Com_Rel.
 Proof.
   eapply Realise_monotone.
-  { unfold App_Tok. TM_Correct.
-    - apply App_Tokens_Realise.
-    - apply Reset_Realise with (X := Tok).
+  { unfold App_Com. TM_Correct.
+    - apply App_Comens_Realise.
+    - apply Reset_Realise with (X := Com).
   }
   { intros tin ((), tout) H. cbn. intros Q t HEncQ HEncT HRight.
-    unfold sigPro, sigTok in *. TMSimp.
+    unfold sigPro, sigCom in *. TMSimp.
     rename H into HNil, H0 into HCons, H1 into HApp, H2 into HReset.
     modpon HNil. modpon HCons. modpon HApp. modpon HReset. repeat split; auto.
   }
 Qed.
 
-Definition App_Tok_steps (Q: Pro) (t:Tok) :=
-  3 + Constr_nil_steps + Constr_cons_steps _ t + App_Tokens_steps Q [t] + Reset_steps _ t.
+Definition App_Com_steps (Q: Pro) (t:Com) :=
+  3 + Constr_nil_steps + Constr_cons_steps _ t + App_Comens_steps Q [t] + Reset_steps _ t.
 
-Definition App_Tok_T : tRel sigPro^+ 3 :=
-  fun tin k => exists (Q: list Tok) (t: Tok), tin[@Fin0] ≃ Q /\ tin[@Fin1] ≃ t /\ isRight tin[@Fin2] /\ App_Tok_steps Q t <= k.
+Definition App_Com_T : tRel sigPro^+ 3 :=
+  fun tin k => exists (Q: list Com) (t: Com), tin[@Fin0] ≃ Q /\ tin[@Fin1] ≃ t /\ isRight tin[@Fin2] /\ App_Com_steps Q t <= k.
 
-Lemma App_Tok_Terminates : projT1 App_Tok ↓ App_Tok_T.
+Lemma App_Com_Terminates : projT1 App_Com ↓ App_Com_T.
 Proof.
   eapply TerminatesIn_monotone.
-  { unfold App_Tok. TM_Correct.
-    - apply App_Tokens_Realise.
-    - apply App_Tokens_Terminates.
-    - apply Reset_Terminates with (X := Tok).
+  { unfold App_Com. TM_Correct.
+    - apply App_Comens_Realise.
+    - apply App_Comens_Terminates.
+    - apply Reset_Terminates with (X := Com).
   }
   {
-    intros tin k (Q&t&HEncQ&HEncT&HRight&Hk). unfold App_Tok_steps in Hk.
-    exists (Constr_nil_steps), (1 + Constr_cons_steps _ t + 1 + App_Tokens_steps Q [t] + Reset_steps _ t). cbn. repeat split; try omega.
+    intros tin k (Q&t&HEncQ&HEncT&HRight&Hk). unfold App_Com_steps in Hk.
+    exists (Constr_nil_steps), (1 + Constr_cons_steps _ t + 1 + App_Comens_steps Q [t] + Reset_steps _ t). cbn. repeat split; try omega.
     intros tmid () (HNil&HInjNil); TMSimp. modpon HNil.
-    exists (Constr_cons_steps _ t), (1 + App_Tokens_steps Q [t] + Reset_steps _ t). cbn. repeat split; try omega.
+    exists (Constr_cons_steps _ t), (1 + App_Comens_steps Q [t] + Reset_steps _ t). cbn. repeat split; try omega.
     eauto. now rewrite !Nat.add_assoc.
     unfold sigPro in *. intros tmid0 () (HCons&HInjCons); TMSimp. modpon HCons.
-    exists (App_Tokens_steps Q [t]), (Reset_steps _ t). cbn. repeat split; try omega.
+    exists (App_Comens_steps Q [t]), (Reset_steps _ t). cbn. repeat split; try omega.
     hnf; cbn. do 2 eexists; repeat split; eauto. reflexivity.
     intros tmid1 _ (HApp&HInjApp); TMSimp. modpon HApp.
     eexists. split; eauto. now setoid_rewrite Reset_steps_comp.
@@ -180,24 +180,24 @@ Qed.
 
 
 Definition JumpTarget_Step : pTM sigPro^+ (option bool) 5 :=
-  If (CaseList sigTok_fin @ [|Fin0; Fin3|])
+  If (CaseList sigCom_fin @ [|Fin0; Fin3|])
      (Switch (ChangeAlphabet CaseCom _ @ [|Fin3|])
-             (fun t : option ATok =>
+             (fun t : option ACom =>
                 match t with
                 | Some retAT =>
                   If (CaseNat ⇑ retr_nat_prog @ [|Fin2|])
-                     (Return (App_ATok retAT @ [|Fin1; Fin4|]) None) (* continue *)
+                     (Return (App_ACom retAT @ [|Fin1; Fin4|]) None) (* continue *)
                      (Return (ResetEmpty1 _ @ [|Fin2|]) (Some true)) (* return true *)
                 | Some lamAT =>
                   Return (Constr_S ⇑ retr_nat_prog @ [|Fin2|];;
-                          App_ATok lamAT @ [|Fin1; Fin4|])
+                          App_ACom lamAT @ [|Fin1; Fin4|])
                          None (* continue *)
                 | Some appAT =>
-                  Return (App_ATok appAT @ [|Fin1;Fin4|])
+                  Return (App_ACom appAT @ [|Fin1;Fin4|])
                          None (* continue *)
                 | None => (* Variable *)
                   Return (Constr_varT ⇑ _ @ [|Fin3|];;
-                          App_Tok @ [|Fin1; Fin3; Fin4|])
+                          App_Com @ [|Fin1; Fin3; Fin4|])
                          None (* continue *)
                 end))
      (Return Nop (Some false)) (* return false *)
@@ -250,12 +250,12 @@ Proof.
   eapply Realise_monotone.
   { unfold JumpTarget_Step. TM_Correct.
     - eapply RealiseIn_Realise. apply CaseCom_Sem.
-    - apply App_ATok_Realise.
+    - apply App_ACom_Realise.
     - eapply RealiseIn_Realise. apply ResetEmpty1_Sem with (X := nat).
-    - apply App_ATok_Realise.
-    - apply App_ATok_Realise.
+    - apply App_ACom_Realise.
+    - apply App_ACom_Realise.
     - eapply RealiseIn_Realise. apply Constr_varT_Sem.
-    - apply App_Tok_Realise.
+    - apply App_Com_Realise.
   }
   {
     intros tin (yout, tout) H. cbn. intros P Q k HEncP HEncQ HEncK HInt3 HInt4.
@@ -300,16 +300,16 @@ Qed.
 
 
 (* Steps after the [CaseCom], depending on [t] *)
-Local Definition JumpTarget_Step_steps_CaseCom (Q: Pro) (k: nat) (t: Tok) :=
+Local Definition JumpTarget_Step_steps_CaseCom (Q: Pro) (k: nat) (t: Com) :=
   match t with
   | retT =>
     match k with
-    | S _ => 1 + CaseNat_steps + App_ATok_steps Q retAT
+    | S _ => 1 + CaseNat_steps + App_ACom_steps Q retAT
     | 0 => 2 + CaseNat_steps + ResetEmpty1_steps
     end
-  | lamT => 1 + Constr_S_steps + App_ATok_steps Q lamAT
-  | appT => App_ATok_steps Q appAT
-  | varT n => 1 + Constr_varT_steps + App_Tok_steps Q t
+  | lamT => 1 + Constr_S_steps + App_ACom_steps Q lamAT
+  | appT => App_ACom_steps Q appAT
+  | varT n => 1 + Constr_varT_steps + App_Com_steps Q t
   end.
 
 (* Steps after the [CaseList] *)
@@ -339,13 +339,13 @@ Proof.
   { unfold JumpTarget_Step. TM_Correct.
     - eapply RealiseIn_Realise. apply CaseCom_Sem.
     - eapply RealiseIn_TerminatesIn. apply CaseCom_Sem.
-    - apply App_ATok_Terminates.
+    - apply App_ACom_Terminates.
     - eapply RealiseIn_TerminatesIn. apply ResetEmpty1_Sem with (X := nat).
-    - apply App_ATok_Terminates.
-    - apply App_ATok_Terminates.
+    - apply App_ACom_Terminates.
+    - apply App_ACom_Terminates.
     - eapply RealiseIn_Realise. apply Constr_varT_Sem.
     - eapply RealiseIn_TerminatesIn. apply Constr_varT_Sem.
-    - apply App_Tok_Terminates.
+    - apply App_Com_Terminates.
   }
   {
     intros tin steps (P&Q&k&HEncP&HEncQ&HEncK&HRight3&HRight4&Hk). unfold JumpTarget_Step_steps in Hk. cbn in *.
@@ -364,16 +364,16 @@ Proof.
           exists ResetEmpty1_steps. repeat split; try omega.
           intros tmid2 bCaseNat (HCaseNat&HCaseNatInj); TMSimp. modpon HCaseNat. destruct bCaseNat; auto.
         - (* k = S k' *)
-          exists (App_ATok_steps Q retAT). repeat split; try omega.
+          exists (App_ACom_steps Q retAT). repeat split; try omega.
           intros tmid2 bCaseNat (HCaseNat&HCaseNatInj); TMSimp. modpon HCaseNat. destruct bCaseNat; auto. hnf; cbn. eauto.
       }
       { (* t = lamT *)
-        exists (Constr_S_steps), (App_ATok_steps Q lamAT). repeat split; try omega.
+        exists (Constr_S_steps), (App_ACom_steps Q lamAT). repeat split; try omega.
         intros tmid2 () (HS&HSInj); TMSimp. modpon HS. hnf; cbn. eauto.
       }
       { (* t = appT *) hnf; cbn; eauto. }
       { (* t = varT n *)
-        exists (Constr_varT_steps), (App_Tok_steps Q (varT n)). repeat split; try omega.
+        exists (Constr_varT_steps), (App_Com_steps Q (varT n)). repeat split; try omega.
         intros tmid2 H (HVarT&HVarTInj); TMSimp. modpon HVarT. hnf; cbn. eauto 6.
       }
     }
@@ -552,7 +552,7 @@ Proof.
   }
   {
     intros tin (yout, tout) H. cbn. intros P HEncP HOut HInt.
-    TMSimp ( unfold sigPro, sigTok in * ). rename H into HWriteNil, H0 into HWriteO, H1 into HLoop.
+    TMSimp ( unfold sigPro, sigCom in * ). rename H into HWriteNil, H0 into HWriteO, H1 into HLoop.
     modpon HWriteNil. modpon HWriteO. modpon HLoop.
     destruct yout.
     - destruct HLoop as (P'&Q'&HLoop); modpon HLoop. do 2 eexists; repeat split; eauto.
